Orderedtree/DOrderedTree/Raw.lean
@@ -3,14 +3,53 @@ Copyright (c) 2024 Lean FRO, LLC. All rights reserved.
 Released under Apache 2.0 license as described in the file LICENSE.
 Authors: Markus Himmel
 -/
+import Orderedtree.DOrderedTree.Internal.Impl
+
+set_option autoImplicit false
+set_option linter.missingDocs true
 
 universe u v
 
-variable {α : Type u} {β : α → Type v}
+variable {α : Type u} {β : α → Type v} {cmp : α → α → Ordering}
 
 namespace Std
 
 namespace DOrderedTree
+
+/-- Binary search trees without a well-formedness invariant, suitable for use in nested inductive
+types. -/
+structure Raw (α : Type u) (β : α → Type v) (_cmp : α → α → Ordering) where
+  /-- Internal implementation detail of the binary search tree. -/
+  inner : Internal.Impl α β
+
+namespace Raw
+
+/-- Unbundled well-formedness invariant for `Raw α β cmp`. -/
+structure WF (l : Raw α β cmp) where
+  /-- Internal implementation detail of the binary search tree. -/
+  out : letI : Ord α := ⟨cmp⟩; l.inner.WF
+
+/-- Creates a new empty binary search tree. -/
+@[inline]
+def empty : Raw α β cmp :=
+  ⟨Internal.Impl.empty⟩
+
+/-- Inserts the mapping `(a, b)` into the binary search tree. -/
+@[inline]
+def insert (l : Raw α β cmp) (a : α) (b : β a) : Raw α β cmp :=
+  letI : Ord α := ⟨cmp⟩; ⟨l.inner.insertSlow a b⟩
+
+/-- Inserts the mapping `(a, b)` into the binary search tree, but faster! -/
+@[inline]
+def insertFast (l : Raw α β cmp) (h : l.WF) (a : α) (b : β a) : Raw α β cmp :=
+  letI : Ord α := ⟨cmp⟩; ⟨(l.inner.insert a b h.out.balanced).impl⟩
+
+/-- Returns `true` if the given key is present in the map. -/
+@[inline]
+def contains (l : Raw α β cmp) (a : α) : Bool :=
+  letI : Ord α := ⟨cmp⟩; l.inner.contains a
+
+end Raw
 
 end DOrderedTree
 
