Orderedtree/DOrderedTree/Basic.lean
@@ -1,0 +1,43 @@
+/-
+Copyright (c) 2024 Lean FRO, LLC. All rights reserved.
+Released under Apache 2.0 license as described in the file LICENSE.
+Authors: Markus Himmel
+-/
+import Orderedtree.DOrderedTree.Internal.Impl
+
+set_option autoImplicit false
+set_option linter.missingDocs true
+
+universe u v
+
+variable {α : Type u} {β : α → Type v} {cmp : α → α → Ordering}
+
+namespace Std
+
+/-- Binary search trees. -/
+structure DOrderedTree (α : Type u) (β : α → Type v) (cmp : α → α → Ordering) where
+  /-- Internal implementation detail of the binary search tree. -/
+  inner : DOrderedTree.Internal.Impl α β
+  /-- Internal implementation detail of the binary search tree. -/
+  wf : letI : Ord α := ⟨cmp⟩; inner.WF
+
+namespace DOrderedTree
+
+/-- Creates a new empty binary search tree. -/
+@[inline]
+def empty : DOrderedTree α β cmp :=
+  letI : Ord α := ⟨cmp⟩; ⟨Internal.Impl.empty, .empty⟩
+
+/-- Inserts the mapping `(a, b)` into the binary search tree, -/
+@[inline]
+def insert (l : DOrderedTree α β cmp) (a : α) (b : β a) : DOrderedTree α β cmp :=
+  letI : Ord α := ⟨cmp⟩; ⟨(l.inner.insert a b l.wf.balanced).impl, .insert l.wf⟩
+
+/-- Returns `true` if the given key is present in the map. -/
+@[inline]
+def contains (l : DOrderedTree α β cmp) (a : α) : Bool :=
+  letI : Ord α := ⟨cmp⟩; l.inner.contains a
+
+end DOrderedTree
+
+end Std
